original haskell compiler is not correct. Corrected compiler and correctness proof

hs-to-coq/examples/compiler/Compiler.hs
@@ -19,10 +19,11 @@ type Code = [Op]
 data Op = PUSH Int | ADD
           deriving Show
 
-exec :: Code -> Stack -> Stack
-exec [] s = s
+exec :: Code -> Stack -> Maybe Stack
+exec [] s = Just s
 exec (PUSH n : c) s = exec c (n : s)
 exec (ADD : c) (m : n : s) = exec c (n+m : s)
+exec (ADD : c) _ = Nothing
 
 comp :: Expr -> Code
 comp (Val n) = [PUSH n]
